\sep

\section{Beweise}
\sep
\subsection{Grundlagen}
\sep

\Beweis $\sup (A + B) \leq \sup A + \sup B$ \\
\(
\text{Es gilt } a + b \leq \sup A + b \leq \sup A + \sup B \\
\implies \sup (A + B) \leq \sup A + \sup B
\)
\sep

\Beweis $\sup A + \sup B \leq \sup(A + B)$  \\
\(
\text{Es gilt } \forall \epsilon > 0 \quad \sup A \leq a -  \frac{\epsilon}{2} \text{ und } \sup B \leq b -  \frac{\epsilon}{2} \\
\implies \sup A + \sup B - \epsilon \leq a + b \leq \sup (A + B) 
\)
\sep

\subsection{Folgen und Reihen}
\sep

\Satz[Sandwich Satz] Wir nehmen an, dass 
\begin{enumerate}
\item $\lim\limits_{n \rightarrow \infty} a_{n} = \lim\limits_{n \rightarrow \infty} b_{n} = \alpha$ 
\item $a_{n} \leq c_{n} \leq b_{n} \ \forall n \geq K$
\end{enumerate}

\(
\text{Es gilt } \abs{a_n - \alpha} < \epsilon \implies - \epsilon < a_n - \alpha \\
\text{Es gilt } \abs{b_n - \alpha} < \epsilon \implies + \epsilon > b_n - \alpha \\
\implies - \epsilon < a_n - \alpha \leq c_n - \alpha \leq b_n - \alpha < \epsilon \\
\implies \abs{c_n - \alpha} < \epsilon \implies \lim\limits_{n \rightarrow \infty} c_{n} = \alpha
\)

\sep

\Beweis $\sum\limits_{k=1}^{\infty} b_k$ konvergiert $ \implies \lim \limits_{n \rightarrow \infty} b_k = 0$
Definiere $c_1 = 0$ mit $c_k = b_{k - 1}$. Es folgt $\sum\limits_{k=1}^{\infty} c_k$ konvergiert und $ \sum\limits_{k=1}^{\infty} b_k = \sum\limits_{k=1}^{\infty} c_k$ 
\[ \implies \lim \limits_{n \rightarrow \infty} b_n = \lim \limits_{n \rightarrow \infty} \Big(\sum\limits_{k= 1}^n b_k - \sum_{k=1}^n c_k \Big ) = 0\]

\sep

\Beweis[Hôpital] $f(c) = g(c) = 0, \quad g'(c) \neq 0$
\begin{align*}
\lim _{x \rightarrow a} \frac{f(x)}{g(x)} &=\lim _{x \rightarrow a} \frac{f(x)-f(a)}{g(x)-g(a)} \\
&=\lim _{x \rightarrow a} \frac{[f(x)-f(a)] /(x-a)}{[g(x)-g(a)] /(x-a)} \\
&=\frac{\lim _{x \rightarrow a}([f(x)-f(a)] /(x-a))}{\lim _{x \rightarrow a}([g(x)-g(a)] /(x-a))} \\
&=\frac{f^{\prime}(a)}{g^{\prime}(a)}
\end{align*}

\sep

\Beweis $\lim \limits_{n \rightarrow \infty} (a_n \cdot b_n) = (\lim \limits_{n \rightarrow \infty} a_n) \cdot (\lim \limits_{n \rightarrow \infty}  b_n)$

Wir dürfen dabei verwenden dass:
\[
\begin{array}{l}
\forall \varepsilon>0 \quad \exists n_{a} \quad \forall n \geq n_{a}:\left|a_{n}-a\right|<\varepsilon \\
\forall \varepsilon>0 \quad \exists n_{b} \quad \forall n \geq n_{b}:\left|b_{n}-b\right|<\varepsilon
\end{array}
\]
Sei also $|a| \geq \varepsilon_{0}>0$ beliebig. Setze $n_{0}:=\max \left\{n_{a}, n_{b}\right\} .$ Dann gilt:
\[
\left|a_{n} b_{n}-a b\right|=\left|a_{n} b_{n}+\left(a_{n} b-a_{n} b\right)-a b\right|
\]
\[
\begin{aligned}
&=\left|a_{n}\left(b_{n}-b\right)+b\left(a_{n}-a\right)\right| \\
(\triangle-\text { Ungl. }) & \leq\left|a_{n}\right|\left|b_{n}-b\right|+|b|\left|a_{n}-a\right| \\
(*),(1),(2) &<(\varepsilon+|a|) \varepsilon+|b| \varepsilon \\
(\varepsilon \leq|a|) & \leq \underbrace{(2|a|+|b|)}_{=: C} \varepsilon=C \cdot \varepsilon \quad\left(\forall n \geq n_{0}\right)
\end{aligned}
\]
\sep